cfrontend/Clight.v
@@ -563,8 +563,8 @@ Inductive step: state -> trace -> state -> Prop :=
       classify_fun (typeof a) = fun_case_f tyargs tyres cconv ->
       eval_expr e le m a vf ->
       eval_exprlist e le m al tyargs vargs ->
-      vf = Vptr fb Ptrofs.zero ->
-      Genv.find_funct ge vf = Some fd ->
+      block_of vf = Some fb ->
+      Genv.find_funct_ptr ge fb = Some fd ->
       type_of_fundef fd = Tfunction tyargs tyres cconv ->
       step (State f (Scall optid a al) k e le m)
         E0 (Callstate fb vargs (Kcall optid f e le k) m)
